src/high/dprop_liftings.v
@@ -1,0 +1,145 @@
+From iris.algebra Require Import auth.
+From iris.bi Require Import fractional.
+From iris.proofmode Require Import reduction monpred tactics.
+
+From self Require Import extra.
+From self.algebra Require Import ghost_map ghost_map_map.
+From self.base Require Import primitive_laws.
+From self.high Require Import dprop monpred_simpl predicates.
+
+Definition lift_d {Σ} P : dProp Σ := with_gnames (λ nD, ⎡ P nD ⎤)%I.
+
+Section lift_d_lemmas.
+  Context {Σ : gFunctors}.
+
+  Lemma lift_wand (P Q : _ → iProp Σ) :
+    (lift_d (λ nD, Q nD -∗ P nD)) -∗
+    (lift_d Q -∗ lift_d P).
+  Proof.
+    iModel. simpl.
+    monPred_simpl.
+    iIntros "impl".
+    iIntros ([??] [? [= <-]]).
+    simpl.
+    monPred_simpl.
+    done.
+  Qed.
+
+  Lemma lift_wand_pure (Q : _ → iProp Σ) P :
+    lift_d (λ nD, Q nD -∗ ⌜ P ⌝) -∗
+    lift_d Q -∗ ⌜ P ⌝.
+  Proof.
+    iModel. simpl.
+    monPred_simpl.
+    iIntros "impl".
+    iIntros ([??] [? [= <-]]).
+    simpl.
+    monPred_simpl.
+    done.
+  Qed.
+
+  Lemma lift_intros (P : _ → iProp Σ) :
+    ⎡ ∀ nD, P nD ⎤ -∗ lift_d P.
+  Proof.
+    iModel. simpl.
+    monPred_simpl.
+    iIntros "impl".
+    iApply "impl".
+  Qed.
+
+End lift_d_lemmas.
+
+(* This tactic eases the proof of lemmas for definitions involving [lift_d].
+   It applies structural rules to turn the goal into one consisting only of assertions in [iProp]. *)
+Ltac lift_d_extract :=
+  iStartProof;
+  rewrite -?lift_wand_pure;
+  rewrite -?lift_wand;
+  rewrite -?lift_intros;
+  iModIntro;
+  iIntros (nD).
+
+Definition crashed_at_d `{nvmBaseFixedG Σ} CV : dProp Σ :=
+  lift_d (λ nD, crashed_at CV)%I.
+
+Definition persisted_loc_d `{nvmBaseFixedG Σ} ℓ t : dProp Σ :=
+  lift_d (λ nD, persisted_loc ℓ t)%I.
+
+Lemma crashed_at_d_agree `{nvmBaseFixedG Σ} CV CV' :
+  crashed_at_d CV -∗ crashed_at_d CV' -∗ ⌜CV = CV'⌝.
+Proof. lift_d_extract. iApply crashed_at_agree. Qed.
+
+Section lemmas.
+  Context `{nvmBaseFixedG Σ}.
+
+  Lemma persisted_loc_d_weak ℓ t1 t2 :
+    t2 ≤ t1 → persisted_loc_d ℓ t1 -∗ persisted_loc_d ℓ t2.
+  Proof.
+    intros le.
+    lift_d_extract.
+    iApply persisted_loc_weak.
+    done.
+  Qed.
+
+End lemmas.
+
+Section post_crash_interact.
+  Context `{nvmG Σ}.
+
+  Context `{AbstractState ST}.
+
+  Definition know_preorder_loc_d `{Countable ST} ℓ (preorder : relation2 ST) : dProp Σ :=
+    lift_d (λ nD, know_preorder_loc ℓ (abs_state_relation (ST := ST)))%I.
+
+  Definition know_pred_d `{Countable ST} ℓ (ϕ : predicate ST) : dProp Σ :=
+    lift_d (λ nD, know_pred ℓ ϕ)%I.
+
+  Definition is_at_loc_d ℓ : dProp Σ :=
+    lift_d (λ nD, own shared_locs_name (◯ {[ ℓ ]}))%I.
+
+  Definition is_na_loc_d ℓ : dProp Σ :=
+    lift_d (λ nD, own exclusive_locs_name (◯ {[ ℓ ]}))%I.
+
+  Definition offset_loc ℓ (t : nat) : dProp Σ :=
+    lift_d (λ nD, ℓ ↪[offset_name]□ t)%I.
+
+  Definition know_na_view_d ℓ q (SV : view) : dProp Σ :=
+    lift_d (λ nD, ℓ ↪[non_atomic_views_gname]{#q} SV)%I.
+
+  Definition know_bumper_d ℓ (bumper : ST → ST) : dProp Σ :=
+    lift_d (λ nD, know_bumper ℓ bumper)%I.
+
+  Definition know_full_history_loc_d `{Countable ST}
+             ℓ q (abs_hist : gmap time ST) : dProp Σ :=
+    lift_d (λ nD, full_entry_unenc abs_history_name ℓ q abs_hist)%I.
+
+  Definition crashed_in_mapsto_d `{Countable ST} ℓ (s : ST) : dProp Σ :=
+    lift_d (λ nD,
+      ∃ es, ⌜ decode es = Some s ⌝ ∗ ℓ ↪[crashed_in_name]□ es)%I.
+
+  Definition know_frag_history_loc_d `{Countable ST} ℓ t (s : ST) : dProp Σ :=
+    lift_d (λ nD, know_frag_history_loc ℓ t s)%I.
+
+  Lemma know_full_entry_frag_entry_unenc ℓ q abs_hist t s :
+    know_full_history_loc_d ℓ q abs_hist -∗
+    know_frag_history_loc_d ℓ t s -∗
+    ⌜ abs_hist !! t = Some s ⌝.
+  Proof.
+    rewrite /know_full_history_loc_d.
+    rewrite /know_frag_history_loc_d.
+    lift_d_extract.
+    iApply full_entry_frag_entry_unenc.
+  Qed.
+
+  Lemma offset_loc_agree ℓ t1 t2 :
+    offset_loc ℓ t1 -∗
+    offset_loc ℓ t2 -∗
+    ⌜ t1 = t2 ⌝.
+  Proof.
+    rewrite /offset_loc.
+    iStartProof.
+    lift_d_extract.
+    iApply (ghost_map_elem_agree _ _ _ _ t1).
+  Qed.
+
+End post_crash_interact.
