src/high/predicates.v
@@ -1,0 +1,326 @@
+From iris.bi Require Import lib.fractional.
+From iris.base_logic.lib Require Import own.
+From iris.algebra Require Import gset gmap excl auth.
+From iris.proofmode Require Import reduction monpred tactics.
+From iris_named_props Require Import named_props.
+
+From self.lang Require Import lang.
+From self.high Require Export resources dprop.
+
+Section predicates.
+  Context `{!nvmG Σ, hGD : nvmDeltaG}.
+
+  (* Note, there are three types for predicates.
+     1/ The real/initial type which depends on some [ST]: *)
+  Definition predicate ST := ST → val → dProp Σ.
+  (* 2/ The encoded type that doesnt depend on [ST]: *)
+  Definition enc_predicate := positive → val → option (dProp Σ).
+  (* 3/ The unwrapped type where we project out of [dProp], forgets that it is
+        monotone, and end up with [thread_view → iProp Σ]: *)
+  Definition unwrapped_predicate :=
+    positive → val → option (thread_view * nvmDeltaG → iProp Σ).
+
+  Definition enc_predicateO :=
+    positive -d> val -d> optionO (dPropO Σ).
+
+  Definition predO :=
+    positive -d> val -d> optionO (thread_view * nvmDeltaG -d> iPropO Σ).
+
+  (* Unfold the [dProp] and forget about monotinicity. *)
+  Definition encoded_pred_unwrap
+    (pred : enc_predicate) : unwrapped_predicate :=
+      λ s v, (λ p i, monPred_at p i) <$> (pred s v).
+
+  Definition encoded_pred_unwrap'
+    (pred : enc_predicateO) : predO :=
+      λ s v, (λ p i, monPred_at p i) <$> (pred s v).
+
+  Definition unwrapped_pred_to_ra (pred : unwrapped_predicate) :
+    (@predicateR Σ) :=
+    to_agree ((λ a b, Next (pred a b))).
+
+  Definition pred_to_ra (pred : enc_predicate) : (@predicateR Σ) :=
+    unwrapped_pred_to_ra (encoded_pred_unwrap pred).
+
+  Global Instance enoded_predc_unwrap :
+    ∀ n, Proper (@dist enc_predicateO _ n ==> @dist predO _ n) encoded_pred_unwrap.
+  Proof.
+    intros ? p1 p2 eq.
+    rewrite /encoded_pred_unwrap.
+    simpl.
+    intros e v.
+    specialize (eq e v).
+    destruct (p1 e v); destruct (p2 e v); simpl;
+      [ |inversion eq|inversion eq|done].
+    apply Some_dist_inj in eq.
+    constructor.
+    intros ?.
+    apply eq.
+  Qed.
+
+  Global Instance pred_to_ra_ne :
+    ∀ n, Proper (@dist enc_predicateO _ n ==> dist n) pred_to_ra.
+  Proof.
+    intros ??? eq.
+    rewrite /pred_to_ra.
+    rewrite /pred_to_ra.
+    rewrite /unwrapped_pred_to_ra.
+    apply (@to_agree_ne (positive -d> val -d> laterO (optionO (index -d> (iPropO Σ))))).
+    intros ??.
+    eassert (NonExpansive Next) as ne; last apply ne; first by apply _.
+    apply enoded_predc_unwrap in eq.
+    specialize (eq x0).
+    apply eq.
+  Qed.
+
+  Definition preds_to_ra (preds : gmap loc (enc_predicate))
+    : gmapUR loc (@predicateR Σ) := pred_to_ra <$> preds.
+
+  Definition own_all_preds dq preds :=
+    own predicates_name (●{dq} (preds_to_ra preds) : predicatesR).
+
+  Definition encode_predicate `{Countable ST} (ϕ : predicate ST)
+    : enc_predicate :=
+    λ encS v, (λ s, ϕ s v) <$> decode encS.
+
+  Definition predicate_to_unwrapped_predicate `{Countable ST} (ϕ : predicate ST)
+    : unwrapped_predicate :=
+    encoded_pred_unwrap (encode_predicate ϕ).
+
+  Definition know_pred `{Countable ST} ℓ (ϕ : predicate ST) : iProp Σ :=
+    own predicates_name
+        (◯ {[ ℓ := unwrapped_pred_to_ra (predicate_to_unwrapped_predicate ϕ) ]}).
+
+  Lemma encode_predicate_extract `{Countable ST}
+      (ϕ : predicate ST) e s v
+      (P : dPropO Σ) i :
+    decode e = Some s →
+    (encode_predicate ϕ e v : optionO (dPropO Σ)) ≡ Some P -∗
+    P i -∗
+    ϕ s v i.
+  Proof.
+    rewrite /encode_predicate.
+    iIntros (->) "equiv".
+    simpl.
+    rewrite option_equivI.
+    iRewrite "equiv".
+    iIntros "$".
+  Qed.
+
+  Lemma encode_predicate_extract_L `{Countable ST}
+        (ϕ : ST → val → dProp Σ) e s v P i :
+    decode e = Some s →
+    encode_predicate ϕ e v = Some P →
+    P i -∗
+    ϕ s v i.
+  Proof. rewrite /encode_predicate. iIntros (-> [= <-]). done. Qed.
+
+  Lemma know_predicates_alloc preds :
+    ⊢ |==> ∃ γ,
+          own γ ((● (pred_to_ra <$> preds)) : predicatesR) ∗
+          own γ ((◯ (pred_to_ra <$> preds)) : predicatesR).
+  Proof.
+    setoid_rewrite <- own_op.
+    iApply own_alloc.
+    apply auth_both_valid_2; last reflexivity.
+    intros ℓ.
+    rewrite lookup_fmap.
+    by case (preds !! ℓ).
+  Qed.
+
+  Lemma encoded_pred_unwrap_inj state v o1 o2 :
+    ⊢@{iPropI Σ} encoded_pred_unwrap o1 state v
+        ≡@{optionO (index -d> iPropO Σ)}
+        encoded_pred_unwrap o2 state v -∗
+      o1 state v ≡@{optionO (dPropO Σ)} o2 state v.
+  Proof.
+    iIntros "#eq".
+    rewrite /encoded_pred_unwrap.
+    destruct o1; destruct o2; simpl;
+      rewrite option_equivI; try done.
+    rewrite option_equivI.
+    rewrite !discrete_fun_equivI.
+    rewrite monPred_equivI. iIntros (i).
+    iApply "eq".
+  Qed.
+
+  Lemma own_all_preds_pred `{Countable ST}
+        dq ℓ (ϕ : predicate ST) (preds : gmap loc enc_predicate) :
+    own_all_preds dq preds -∗
+    know_pred ℓ ϕ -∗
+    (∃ (o : enc_predicateO),
+       ⌜preds !! ℓ = Some o⌝ ∗ (* Some encoded predicate exists. *)
+       ▷ (o ≡ encode_predicate ϕ)).
+  Proof.
+    iIntros "O K".
+    iDestruct (own_valid_2 with "O K") as "H".
+    iDestruct (auth_both_dfrac_validI with "H") as "(_ & tmp & val)".
+    iDestruct "tmp" as (c) "#eq".
+    rewrite gmap_equivI.
+    iSpecialize ("eq" $! ℓ).
+    rewrite lookup_fmap.
+    rewrite lookup_op.
+    rewrite lookup_singleton.
+    destruct (preds !! ℓ) as [o|] eqn:eq; simpl.
+    2: { simpl. case (c !! ℓ); intros; iDestruct "eq" as %eq'; inversion eq'. }
+    iExists o.
+    iSplit; first done.
+    case (c !! ℓ).
+    - intros ?.
+      rewrite -Some_op.
+      rewrite !option_equivI.
+      rewrite wsat.agree_equiv_inclI.
+      rewrite !discrete_fun_equivI. iIntros (state).
+      iSpecialize ("eq" $! state).
+      rewrite !discrete_fun_equivI. iIntros (v).
+      iSpecialize ("eq" $! v).
+      rewrite later_equivI_1.
+      iNext.
+      rewrite /predicate_to_unwrapped_predicate.
+      iDestruct (encoded_pred_unwrap_inj with "eq") as "eq2".
+      iRewrite "eq2".
+      done.
+    - rewrite right_id.
+      simpl.
+      rewrite !option_equivI.
+      rewrite agree_equivI.
+      rewrite !discrete_fun_equivI. iIntros (state).
+      iSpecialize ("eq" $! state).
+      rewrite !discrete_fun_equivI. iIntros (v).
+      iSpecialize ("eq" $! v).
+      rewrite later_equivI_1.
+      iNext.
+      rewrite /predicate_to_unwrapped_predicate.
+      iDestruct (encoded_pred_unwrap_inj with "eq") as "eq2".
+      done.
+  Qed.
+
+  Lemma predicates_frag_lookup γ predicates (ℓ : loc) pred :
+    predicates !! ℓ = Some pred →
+    own γ (◯ (pred_to_ra <$> predicates) : predicatesR) -∗
+    own γ (◯ {[ ℓ := pred_to_ra pred ]}).
+  Proof.
+    intros look. f_equiv. simpl.
+    apply auth_frag_mono.
+    rewrite singleton_included_l.
+    eexists _.
+    rewrite lookup_fmap look.
+    naive_solver.
+  Qed.
+
+  (** If [pred] is the encoding of [Φ] then [pred] holding for the encoding of
+  [s] is equivalent to [ϕ] holding for [s]. *)
+  Lemma pred_encode_Some `{Countable ST}
+        ϕ (s : ST) (v : val) (pred : enc_predicateO) :
+    (pred ≡ encode_predicate ϕ : iProp Σ) -∗
+    (pred (encode s) v ≡ Some (ϕ s v) : iProp Σ).
+  Proof.
+    iIntros "eq".
+    iEval (setoid_rewrite discrete_fun_equivI) in "eq".
+    iEval (setoid_rewrite discrete_fun_equivI) in "eq".
+    iSpecialize ("eq" $! (encode s) v).
+    Unshelve. 2: { done. } 2: { done. }
+    rewrite /encode_predicate. rewrite decode_encode /=.
+    done.
+  Qed.
+
+  Lemma own_all_preds_insert `{Countable ST} preds ℓ (ϕ : ST → val → dProp Σ) :
+    preds !! ℓ = None →
+    own predicates_name (● preds_to_ra preds) ==∗
+    own predicates_name (● preds_to_ra (<[ℓ := encode_predicate ϕ]>preds)) ∗
+    know_pred ℓ ϕ.
+  Proof.
+    iIntros (look) "A".
+    rewrite /know_pred.
+    rewrite comm.
+    iMod (own_update with "A") as "[H $]".
+    { apply auth_update_alloc.
+      apply alloc_local_update; last done.
+      rewrite /preds_to_ra. rewrite lookup_fmap. erewrite look. done. }
+    iModIntro.
+    rewrite /preds_to_ra.
+    rewrite fmap_insert.
+    iFrame.
+  Qed.
+
+End predicates.
+
+Section encoded_predicate.
+  Context `{AbstractState ST}.
+  Context `{!nvmG Σ}.
+
+  Implicit Types (s : ST) (ϕ : ST → val → dProp Σ).
+
+  Definition encoded_predicate_holds
+    (enc_pred : positive → val → optionO (dPropO Σ))
+    (enc_state : positive) (v : val) i : iProp Σ :=
+    (∃ P, (enc_pred enc_state v ≡ Some P) ∗ P i).
+
+  Lemma predicate_holds_phi_decode ϕ s encS (encϕ : enc_predicateO) v i :
+    decode encS = Some s →
+    (encϕ ≡ encode_predicate ϕ)%I -∗
+    (encoded_predicate_holds encϕ encS v i ∗-∗ ϕ s v i).
+  Proof.
+    iIntros (eq') "predsEquiv".
+    iSplit.
+    - iDestruct 1 as (P') "[eq PH]".
+      iDestruct (discrete_fun_equivI with "predsEquiv") as "HI".
+      iDestruct ("HI" $! encS) as "HIP". (* iClear "HI". *)
+      iEval (rewrite discrete_fun_equivI) in "HIP".
+      iDestruct ("HIP" $! v) as "HI". (* iClear "HIP". *)
+      rewrite /encode_predicate.
+      rewrite eq'.
+      simpl.
+      iRewrite "eq" in "HI".
+      rewrite option_equivI.
+      by iRewrite "HI" in "PH".
+    - iIntros "phi".
+      rewrite /encoded_predicate_holds.
+      do 2 iEval (setoid_rewrite discrete_fun_equivI) in "predsEquiv".
+      iSpecialize ("predsEquiv" $! encS v).
+      rewrite /encode_predicate. rewrite eq'.
+      simpl.
+      destruct (encϕ encS v); rewrite option_equivI; last done.
+      iExists _. iSplit; first done.
+      by iRewrite "predsEquiv".
+  Qed.
+
+  Lemma predicate_holds_phi_decode_1 ϕ s encS (encϕ : enc_predicateO) v i :
+    decode encS = Some s →
+    (encϕ ≡ encode_predicate ϕ)%I -∗
+    (encoded_predicate_holds encϕ encS v i -∗ ϕ s v i).
+  Proof.
+    iIntros (?) "H1 H2".
+    iApply (predicate_holds_phi_decode with "H1 H2").
+    done.
+  Qed.
+
+  Lemma predicate_holds_phi_decode_2 ϕ s encS (encϕ : enc_predicateO) v i :
+    decode encS = Some s →
+    (encϕ ≡ encode_predicate ϕ)%I -∗
+    ϕ s v i -∗
+    encoded_predicate_holds encϕ encS v i.
+  Proof.
+    iIntros (?) "H1 H2".
+    iApply (predicate_holds_phi_decode with "H1 H2").
+    done.
+  Qed.
+
+  Lemma predicate_holds_phi ϕ s encS (encϕ : enc_predicateO) v i :
+    encS = encode s →
+    (encϕ ≡ encode_predicate ϕ)%I -∗
+    (encoded_predicate_holds encϕ encS v i ∗-∗ ϕ s v i).
+  Proof.
+    iIntros (eqEncS) "predsEquiv".
+    iApply predicate_holds_phi_decode; last done.
+    rewrite eqEncS. apply decode_encode.
+  Qed.
+
+  Global Instance encoded_predicate_holds_mono encϕ encS v :
+    Proper ((⊑) ==> (⊢)) (encoded_predicate_holds encϕ encS v).
+  Proof.
+    iIntros (???). iDestruct 1 as (P) "[eq P]".
+    iExists P. iFrame.
+  Qed.
+
+End encoded_predicate.
